x86/RelocProgSemantics2.v
@@ -88,7 +88,8 @@ Fixpoint decode_instrs (fuel:nat) (ofs: Z) (bytes: list byte) (instrs: list inst
   end.
 
 Definition decode_instrs' (bytes: list byte) :=
-  decode_instrs (length bytes) 0 bytes nil.
+  do instrs <- decode_instrs (length bytes) 0 bytes nil;
+  OK (rev instrs).
   
 Definition decode_code_section (s:section) : res section :=
   match s with
